SepAuto: improvement in step speed. ADestructPair, DestructVarname: files for step speed improvement. AByteFile: Complete: write_to_block_ok.     Almost Complete: grow_ok, write_middle_blocks_ok, dwrite_first_block_ok.

src/AByteFile.v
@@ -79,7 +79,12 @@ Definition mem_except_range AEQ V (m: @Mem.mem _ AEQ V) a n :=
             then None 
            else m a'
     else m a').
-
+    
+Fixpoint list_split_chunk A k cs (l: list A): list (list A) :=
+match k with
+  | O => nil
+  | S k' => (firstn cs l)::(list_split_chunk k' cs (skipn cs l))
+end.
 
 (* rep invariants *)
 Definition proto_bytefile_valid f pfy: Prop :=
@@ -260,13 +265,19 @@ Definition write_to_block lxp ixp inum fms block_off byte_off data :=
 Definition write_middle_blocks lxp ixp inum fms block_off num_of_full_blocks data:=
    ms <- ForN i < num_of_full_blocks
         Hashmap hm 
-        Ghost [crash F Fd m0 m]
+        Ghost [crash F Fi Fm bxp frees ilist]
         Loopvar [ms']
         Invariant 
-          exists fy,
-          LOG.rep lxp F (LOG.ActiveTxn m0 m) (BFILE.MSLL ms') hm *
+          exists m0' m' flist Fd Fx f fy,
+          LOG.rep lxp F (LOG.ActiveTxn m0' m') (BFILE.MSLL ms') hm *
+          [[[ m' ::: (Fm * BFILE.rep bxp ixp flist ilist frees) ]]] *
+          [[[ flist ::: (Fi * inum |-> f) ]]] *
+          [[ length (ByFData fy) >= (block_off + i) * valubytes + valubytes]] *
+          rep f fy *
+          [[[ (BFILE.BFData f):::(Fx * arrayN (ptsto (V:= valuset)) (block_off) (map (fun x => (list2valu x,nil)) (list_split_chunk i valubytes (get_sublist data 0 (i*valubytes)))))]]] * 
           [[[ (ByFData fy)::: 
               (Fd * arrayN (ptsto (V:=byteset)) (block_off * valubytes) (map (fun x => (x,nil)) (get_sublist data 0 (i*valubytes)%nat)))]]] *
+          [[ forall i, i < length (ByFData fy) -> snd (selN (ByFData fy) i byteset0) = nil ]] *
           [[ BFILE.MSAlloc fms = BFILE.MSAlloc ms' ]]
         OnCrash crash
         Begin (
@@ -278,7 +289,7 @@ Definition write_middle_blocks lxp ixp inum fms block_off num_of_full_blocks dat
 
 
 
-(* Definition dwrite_to_block lxp ixp inum fms block_off byte_off data :=
+Definition dwrite_to_block lxp ixp inum fms block_off byte_off data :=
     let^ (fms, block) <- BFILE.read lxp ixp inum block_off fms;   (* get the block *) 
     let block_list := valu2list block in
     let block_write := list2valu ((firstn byte_off block_list)     (* Construct new block*)
@@ -287,7 +298,7 @@ Definition write_middle_blocks lxp ixp inum fms block_off num_of_full_blocks dat
   Ret (fms).
   
 
-Definition dwrite_middle_blocks lxp ixp inum fms block_off num_of_full_blocks data:=
+(* Definition dwrite_middle_blocks lxp ixp inum fms block_off num_of_full_blocks data:=
    ms <- ForN i < num_of_full_blocks
         Hashmap hm 
         Ghost [crash F Fm Fi bxp flist ilist frees m0 m f]
@@ -342,15 +353,16 @@ Definition updattr := BFILE.updattr.
 Definition datasync := BFILE.datasync.
 Definition sync := BFILE.sync.
     
-(* Definition grow lxp bxps ixp inum b fms :=
-    let^ (ms, len) <- getlen lxp ixp inum fms;
-    If (Nat.eq_dec 0 (len mod valubytes)) (* no room in the block *)
+Definition grow lxp bxps ixp inum b fms :=
+    let^ (bms, bylen) <- getlen lxp ixp inum fms;
+    let^ (ms, blen) <- BFILE.getlen lxp ixp inum bms;
+    If (Nat.eq_dec bylen (blen*valubytes)) (* no room in the block *)
     {
-        let^ (ms', res) <- BFILE.grow lxp bxps ixp inum (byte2valu b) fms;
+        let^ (ms', res) <- BFILE.grow lxp bxps ixp inum (byte2valu b) ms;
         If (bool_dec res true)
         {
-          ms'' <- (*ADD: update size *)
-          Ret ^(BFILE.mk_memstate ms'' (BFILE.MSLL ms'), res)
+          ms'' <- BFILE.updattr lxp ixp inum (INODE.UBytes $(S bylen)) ms';(*ADD: update size *)
+          Ret ^(ms'', res)
         }
         else
         {
@@ -359,13 +371,98 @@ Definition sync := BFILE.sync.
      }
      else
      {
-       ms' <- write lxp ixp inum len (b::nil) ms;
-       ms'' <- (*ADD: update size *)
-       Ret ^(BFILE.mk_memstate ms'' (BFILE.MSLL ms'), true)
+       ms' <- write_to_block lxp ixp inum ms (bylen/valubytes) (bylen mod valubytes) (b::nil);
+       ms'' <- BFILE.updattr lxp ixp inum (INODE.UBytes $(S bylen)) ms'; (*ADD: update size *)
+       Ret ^(ms'', true)
      }.
- *)
+     
  
 (* Helper lemmas.*)
+Lemma diskIs_id: forall AT AEQ V (m:Mem.mem), @diskIs AT AEQ V m m.
+Proof. intros; unfold diskIs; reflexivity. Qed.
+
+Lemma addr_id: forall A (l: list A) a def, 
+a < length l ->
+((diskIs (mem_except (list2nmem l) a)) * a |-> (selN l a def))%pred (list2nmem l).
+Proof.
+intros.
+eapply diskIs_extract.
+eapply list2nmem_ptsto_cancel in H.
+pred_apply; cancel.
+firstorder.
+Qed.
+
+Lemma mem_except_range_O: forall AEQ V (m: @Mem.mem _ AEQ V) a,
+mem_except_range m a 0 = m.
+Proof.
+intros.
+unfold mem_except_range.
+rewrite <- plus_n_O.
+apply functional_extensionality.
+intros.
+destruct (le_dec a x);
+destruct (lt_dec x a); try omega; try reflexivity.
+Qed.
+
+Definition ext_opt T (ov: option T) def :=
+match ov with
+| None => def
+| Some v => v
+end.
+
+Fact out_except_range_then_in: forall (l: list valuset) s a n def,
+a < length l ->
+a < s \/ a >= s + n ->
+(exists F0 : pred, (sep_star (AEQ:= addr_eq_dec) F0 (a |-> ext_opt ((list2nmem l) a) def))%pred (@mem_except_range addr_eq_dec valuset (list2nmem l) s n)).
+Proof.
+intros.
+eexists.
+apply sep_star_comm.
+apply mem_except_ptsto with (a:= a).
+unfold mem_except_range.
+destruct H0.
+destruct (le_dec s a); try omega.
+unfold list2nmem, ext_opt.
+erewrite selN_map.
+reflexivity. auto.
+destruct (lt_dec a (s + n)); try omega.
+destruct (le_dec s a); try omega.
+unfold list2nmem, ext_opt.
+erewrite selN_map.
+reflexivity. auto.
+instantiate (1:= diskIs (mem_except (mem_except_range (list2nmem l) s n) a)).
+apply diskIs_id.
+Grab Existential Variables.
+apply valuset0.
+apply valuset0.
+Qed.
+
+Fact mem_ex_mem_ex_range: forall (A: Type) AEQ i j (l: list A),
+mem_except (AEQ:= AEQ) (mem_except_range (list2nmem l) i j) (i + j) = mem_except_range (list2nmem l) i (j + 1).
+Proof.
+intros.
+unfold mem_except, mem_except_range.
+apply functional_extensionality; intros.
+destruct (AEQ x (i + j)).
+rewrite e.
+destruct (le_dec i (i + j)).
+destruct (lt_dec (i + j) (i + (j + 1))).
+reflexivity.
+omega.
+omega.
+
+destruct (le_dec i x).
+destruct (lt_dec x (i + j)).
+destruct (lt_dec x (i + (j + 1))).
+reflexivity.
+omega.
+destruct (lt_dec x (i + (j + 1))).
+omega.
+reflexivity.
+reflexivity.
+Qed.
+
+
 Lemma block_content_match: forall F f vs block_off def, 
 (F * block_off|-> vs)%pred (list2nmem(BFILE.BFData f))-> 
 vs = selN (BFILE.BFData f) block_off def.
@@ -404,19 +501,6 @@ rewrite H.
 rewrite firstn_length.
 rewrite flat_map_len.
 apply Min.le_min_r.
-Qed.
-
-
-Lemma addr_id: forall A (l: list A) a def, 
-a < length l ->
-((diskIs (mem_except (list2nmem l) a)) * a |-> (selN l a def))%pred (list2nmem l).
-
-Proof.
-intros.
-eapply diskIs_extract.
-eapply list2nmem_ptsto_cancel in H.
-pred_apply; cancel.
-firstorder.
 Qed.
 
 Lemma bytefile_unified_byte_len: forall ufy fy, 
@@ -768,51 +852,6 @@ sepauto.
 Qed.
 
 
-Fact minus_eq_O: forall n m, n >= m -> n - m = 0 -> n = m.
-Proof.
-induction n; intros.
-inversion H; reflexivity.
-destruct m.
-inversion H0.
-apply eq_S.
-apply IHn.
-omega. omega.
-Qed.
-
-Fact valubytes_ne_O: valubytes <> 0.
-Proof. rewrite valubytes_is; unfold not; intros H'; inversion H'. Qed.
-
-Fact divmult_plusminus_eq:forall n m, m <> 0 ->
-   m + n / m * m = n + (m - n mod m).
-Proof.
-intros.   
-rewrite Nat.add_sub_assoc.
-replace (n + m - n mod m) 
-    with (m + n - n mod m) by omega.
-rewrite <- Nat.add_sub_assoc.
-rewrite Nat.add_cancel_l with (p:= m); eauto.
-rewrite Nat.mod_eq; eauto.
-rewrite Rounding.sub_sub_assoc.
-apply Nat.mul_comm.
-apply Nat.mul_div_le; eauto.
-apply Nat.mod_le; eauto.
-apply Nat.lt_le_incl.
-apply Nat.mod_upper_bound; eauto.
-Qed.
-
-Fact le_minus_divmult: forall n m k, m <> 0 ->
-    n - (m - k mod m) - (n - (m - k mod m)) / m * m <= m.
-Proof. intros.
-remember (n - (m - k mod m)) as b.
-replace (b - b / m * m) with (b mod m).
-apply Nat.lt_le_incl.
-apply Nat.mod_upper_bound; eauto.
-rewrite Nat.mul_comm.
-apply Nat.mod_eq; eauto.
-Qed.
-
-Fact grouping_minus: forall n m k a, n - (m - k + a) = n - (m - k) - a.
-Proof. intros. omega. Qed.
 
 Fact flist_eq_ilist: forall F F' flist flist' ilist m, 
   (@sep_star addr addr_eq_dec BFILE.datatype 
@@ -840,36 +879,6 @@ Proof.
   Grab Existential Variables.
   apply O.
 Qed.
-
-
-Fact map_1to1_eq: forall A B (f: A -> B) (l l': list A), 
-  (forall x y, f x = f y -> x = y) -> 
-  map f l = map f l' ->
-  l = l'.
-  
-Proof.
-  induction l; intros.
-  simpl in H0; symmetry in H0.
-  eapply map_eq_nil in H0.
-  eauto.
-  destruct l'.
-  rewrite map_cons in H0; simpl in H0.
-  inversion H0.
-  repeat rewrite map_cons in H0.
-  inversion H0.
-  apply H in H2.
-  rewrite H2.
-  eapply IHl in H.
-  apply cons_simpl.
-  eauto.
-  eauto.
-Qed.
-
-Fact map_eq: forall A B (f: A -> B) (l l': list A), 
-  l = l' ->
-  map f l = map f l'.
-
-Proof. intros; rewrite H; reflexivity. Qed.
 
 
 Fact unibyte_len: forall f pfy ufy fy i,
@@ -935,156 +944,14 @@ auto.
 auto.
 Qed.
 
-
-Lemma diskIs_id: forall AT AEQ V (m:Mem.mem), @diskIs AT AEQ V m m.
-Proof. intros; unfold diskIs; reflexivity. Qed.
-
-Lemma mem_except_range_O: forall AEQ V (m: @Mem.mem _ AEQ V) a,
-mem_except_range m a 0 = m.
-Proof.
-intros.
-unfold mem_except_range.
-rewrite <- plus_n_O.
-apply functional_extensionality.
-intros.
-destruct (le_dec a x);
-destruct (lt_dec x a); try omega; try reflexivity.
-Qed.
-
-Lemma le_mult_weaken: forall p n m, p > 0 -> n * p <= m * p  -> n <= m.
-Proof.
-  assert(A: forall x, 0 * x = 0). intros. omega.
-  induction n. intros.
-  destruct m.
-  omega.
-  omega. intros.
-  destruct m.
-  inversion H0.
-  apply plus_is_O in H2.
-  destruct H2.
-  omega.
-  apply le_n_S.
-  apply IHn.
-  auto.
-  simpl in H0.
-  omega.
-Qed.
-
-Definition ext_opt T (ov: option T) def :=
-match ov with
-| None => def
-| Some v => v
-end.
-
-Fact out_except_range_then_in: forall (l: list valuset) s a n def,
-a < length l ->
-a < s \/ a >= s + n ->
-(exists F0 : pred, (sep_star (AEQ:= addr_eq_dec) F0 (a |-> ext_opt ((list2nmem l) a) def))%pred (@mem_except_range addr_eq_dec valuset (list2nmem l) s n)).
-Proof.
-intros.
-eexists.
-apply sep_star_comm.
-apply mem_except_ptsto with (a:= a).
-unfold mem_except_range.
-destruct H0.
-destruct (le_dec s a); try omega.
-unfold list2nmem, ext_opt.
-erewrite selN_map.
-reflexivity. auto.
-destruct (lt_dec a (s + n)); try omega.
-destruct (le_dec s a); try omega.
-unfold list2nmem, ext_opt.
-erewrite selN_map.
-reflexivity. auto.
-instantiate (1:= diskIs (mem_except (mem_except_range (list2nmem l) s n) a)).
-apply diskIs_id.
-Grab Existential Variables.
-apply valuset0.
-apply valuset0.
-Qed.
-
-
-Fact vs2bs_selN_O: forall l,
-selN (valuset2bytesets l) 0 byteset0 = (list2byteset byte0 (map (selN' 0 byte0) (map valu2list (byteset2list l)))).
-Proof.
-intros.
-unfold valuset2bytesets.
-destruct l.
-simpl.
-rewrite map_map; simpl.
-rewrite valuset2bytesets_rec_expand.
-simpl.
-unfold selN'.
-rewrite map_map; reflexivity.
-rewrite valubytes_is; omega.
-Qed.
-
-Lemma updN_eq: forall A v v' a (l: list A), v = v' -> updN l a v  = updN l a v'.
-Proof. intros; subst; reflexivity. Qed.
-
-Lemma skipn_concat_skipn: forall A j i k (l: list (list A)) def,
-i <= k -> j < length l -> Forall (fun sublist : list A => length sublist = k) l ->
-skipn i (concat (skipn j l)) = skipn i (selN l j def) ++ concat (skipn (S j) l).
-Proof. induction j; destruct l; intros; simpl.
-inversion H0.
-apply skipn_app_l.
-rewrite Forall_forall in H1.
-destruct H1 with (x:= l).
-apply in_eq.
-omega.
-inversion H0.
-erewrite IHj.
-reflexivity.
-eauto.
-simpl in H0; omega.
-eapply Forall_cons2.
-eauto.
-Qed.
-
-
-Fact mem_ex_mem_ex_range: forall (A: Type) AEQ i j (l: list A),
-mem_except (AEQ:= AEQ) (mem_except_range (list2nmem l) i j) (i + j) = mem_except_range (list2nmem l) i (j + 1).
-Proof.
-intros.
-unfold mem_except, mem_except_range.
-apply functional_extensionality; intros.
-destruct (AEQ x (i + j)).
-rewrite e.
-destruct (le_dec i (i + j)).
-destruct (lt_dec (i + j) (i + (j + 1))).
-reflexivity.
-omega.
-omega.
-
-destruct (le_dec i x).
-destruct (lt_dec x (i + j)).
-destruct (lt_dec x (i + (j + 1))).
-reflexivity.
-omega.
-destruct (lt_dec x (i + (j + 1))).
-omega.
-reflexivity.
-reflexivity.
-Qed.
-
-Lemma le_le_weaken: forall n m p k,
-n + m <= p -> k <= m -> n + k <= p.
-Proof. intros.
-omega.
-Qed.
-
-Lemma le_lt_weaken: forall n m p k,
-n + m <= p -> k < m -> n + k < p.
-Proof. intros.
-omega.
-Qed.
-
-Fact inbound_protobyte: forall f pfy ufy fy block_off m1 data Fd,
+Fact inbound_protobyte: forall f pfy ufy fy block_off m1 nb data Fd,
 proto_bytefile_valid f pfy ->
 unified_bytefile_valid pfy ufy ->
 bytefile_valid ufy fy ->
 (Fd ✶ arrayN (ptsto (V:=byteset)) (block_off * valubytes) data)%pred (list2nmem (ByFData fy)) -> 
-length data > m1 * valubytes ->
+nb > 0 ->
+length data = nb * valubytes ->
+m1 < nb ->
 block_off + m1 < length (PByFData pfy).
 Proof.
 intros.
@@ -1092,21 +959,1008 @@ rewrite H.
 rewrite map_length.
 apply list2nmem_arrayN_bound in H2 as H'.
 destruct H'.
-rewrite <- length_zero_iff_nil in H4.
-rewrite H4 in H3; inversion H3.
-rewrite bytefile_unified_byte_len with (ufy:= ufy) in H4; eauto.
-rewrite unified_byte_protobyte_len with (pfy:= pfy)(k:=valubytes) in H4; eauto.
-eapply le_lt_weaken in H4; eauto.
-rewrite <- Nat.mul_add_distr_r in H4.
-apply lt_mult_weaken in H4.
-rewrite H in H4.
-rewrite map_length in H4.
+rewrite <- length_zero_iff_nil in H6.
+rewrite H6 in H4; symmetry in H4; apply mult_is_O in H4.
+destruct H4.
+omega.
+rewrite valubytes_is in *; omega.
+apply list2nmem_arrayN_bound in H2.
+destruct H2.
+apply length_zero_iff_nil in H2; rewrite valubytes_is in *; omega.
+
+
+rewrite bytefile_unified_byte_len with (ufy:= ufy) in H6; eauto.
+rewrite unified_byte_protobyte_len with (pfy:= pfy)(k:=valubytes) in H6; eauto.
+rewrite H4 in H6.
+eapply le_lt_weaken with (k:= m1 * valubytes) in H6; eauto.
+rewrite <- Nat.mul_add_distr_r in H6.
+apply lt_mult_weaken in H6.
+rewrite H in H6.
+rewrite map_length in H6.
 auto.
+rewrite valubytes_is in *; omega.
 eapply proto_len; eauto.
 Qed.
 
 
+Lemma exists_unique_bytefile_length: forall f pfy ufy fy,
+proto_bytefile_valid f pfy ->
+unified_bytefile_valid pfy ufy ->
+bytefile_valid ufy fy ->
+length (ByFData fy) mod valubytes = 0 ->
+length (ByFData fy) > 0 ->
+exists ! x, length (ByFData fy) = x * valubytes.
+Proof.
+intros.
+unfold unique.
+apply Nat.mod_divides in H2; destruct H2.
+exists x.
+split.
+rewrite Nat.mul_comm; auto.
+intros.
+rewrite H2 in H4.
+rewrite Nat.mul_comm in H4.
+apply Nat.mul_cancel_r in H4; auto.
+apply valubytes_ne_O.
+unfold not; intros.
+unfold not in *; apply mod_dem_neq_dem with (a:= length (ByFData fy)) (b:= valubytes); intros; rewrite valubytes_is in *; omega.
+Qed.
+
+
+Lemma bfile_protobyte_len_eq: forall f pfy,
+  proto_bytefile_valid f pfy ->
+  length (PByFData pfy) = length (BFILE.BFData f).
+Proof.
+intros.
+rewrite H.
+apply map_length.
+Qed.
+
+Lemma map_same: forall A B (l1 l2: list A) (f: A -> B),
+l1 = l2 -> map f l1 = map f l2.
+Proof. intros; subst; reflexivity. Qed.
+
+Lemma list2nmem_arrayN_middle: forall A  (l2 l1 l3: list A) (F:pred),
+F (mem_except_range (list2nmem (l1 ++ l2 ++ l3)) (length l1) (length l2) ) -> (F * arrayN (ptsto (V:= A)) (length l1) l2)%pred (list2nmem (l1 ++ l2 ++ l3)).
+Proof.
+induction l2; intros.
+simpl.
+apply emp_star_r.
+unfold mem_except_range in H.
+rewrite app_assoc in H.
+rewrite app_nil_r in H.
+simpl in H.
+rewrite <- plus_n_O in H.
+replace (list2nmem (l1 ++ l3)) with 
+        (fun a' : addr =>
+       if le_dec (length l1) a' then if lt_dec a' (length l1) then None else list2nmem (l1 ++ l3) a' else list2nmem (l1 ++ l3) a').
+auto.
+apply functional_extensionality; intros.
+destruct (le_dec (length l1) x);
+destruct (lt_dec x (length l1)); try reflexivity.
+omega.
+
+rewrite arrayN_isolate with (i := 0).
+simpl.
+apply sep_star_assoc.
+replace (length l1 + 0 + 1) with (length (l1 ++ a :: nil)).
+replace (l1 ++ a :: l2 ++ l3) with ((l1 ++ (a :: nil)) ++ l2 ++ l3).
+apply IHl2 with (F:= (F ✶ (emp ✶ (length l1 + 0) |-> a))%pred).
+auto.
+apply sep_star_assoc.
+apply sep_star_comm.
+apply mem_except_ptsto.
+rewrite <- plus_n_O.
+unfold list2nmem.
+unfold mem_except_range.
+erewrite selN_map.
+rewrite selN_app.
+rewrite selN_app2.
+replace (length l1 - length l1) with 0 by omega.
+simpl.
+rewrite app_length; simpl.
+destruct (le_dec (length l1 + 1) (length l1)); try omega; try reflexivity.
+omega.
+rewrite app_length; simpl; omega.
+repeat rewrite app_length; simpl; omega.
+apply emp_star_r.
+unfold mem_except, mem_except_range.
+rewrite <- plus_n_O.
+repeat rewrite app_length in *; simpl in *.
+replace (fun a' : addr =>
+   if addr_eq_dec a' (length l1)
+   then None
+   else
+    if le_dec (length l1 + 1) a'
+    then if lt_dec a' (length l1 + 1 + length l2) then None else list2nmem ((l1 ++ a :: nil) ++ l2 ++ l3) a'
+    else list2nmem ((l1 ++ a :: nil) ++ l2 ++ l3) a')
+    
+with (mem_except_range (list2nmem (l1 ++ a :: l2 ++ l3)) (length l1) (S (length l2))).
+auto.
+unfold mem_except_range.
+apply functional_extensionality; intros.
+
+replace ((length l1 + 1 + length l2)) with (length l1 + S (length l2)) by omega.
+replace (((l1 ++ a :: nil) ++ l2 ++ l3)) with (l1 ++ a :: l2 ++ l3).
+
+destruct (le_dec (length l1 + 1) x);
+destruct (le_dec (length l1) x);
+destruct (addr_eq_dec x (length l1)); try omega; try reflexivity.
+destruct (lt_dec x (length l1 + S (length l2))); try omega; try reflexivity.
+
+rewrite <- app_assoc.
+rewrite <- cons_app.
+reflexivity.
+
+rewrite <- app_assoc.
+rewrite <- cons_app.
+reflexivity.
+
+rewrite app_length; simpl; omega.
+simpl; omega.
+
+Unshelve.
+auto.
+Grab Existential Variables.
+auto.
+Qed. 
+
+Lemma arrayN_frame_mem_ex_range: forall A (l: list A) (F:pred) a m,
+(F * arrayN (ptsto (V:= A)) a l)%pred m -> F (mem_except_range m a (length l) ).
+Proof.
+induction l; intros.
+simpl in *.
+unfold mem_except_range.
+rewrite <- plus_n_O.
+replace ((fun a' : addr => if le_dec a a' then if lt_dec a' a then None else m a' else m a')) with m.
+apply sep_star_comm in H.
+apply star_emp_pimpl in H; auto.
+apply functional_extensionality; intros.
+destruct (le_dec a x);
+destruct (lt_dec x a);
+try omega; try reflexivity.
+replace (mem_except_range m a0 (length (a :: l))) with (mem_except_range (mem_except m a0) (a0 + 1) (length l)).
+apply IHl.
+rewrite isolateN_fwd with (i:= 0) in H; simpl in H.
+rewrite star_emp_pimpl in H.
+rewrite <- plus_n_O in H.
+apply sep_star_comm in H.
+apply sep_star_assoc in H.
+apply ptsto_mem_except in H. pred_apply; cancel.
+simpl; omega.
+apply functional_extensionality; intros.
+unfold mem_except, mem_except_range; simpl.
+replace (S (length l)) with ( 1 + length l) by omega.
+rewrite Nat.add_assoc.
+destruct (le_dec (a0 + 1) x);
+destruct (lt_dec x (a0 + 1 + length l));
+destruct (addr_eq_dec x a0);
+destruct (le_dec a0 x);
+try omega; try reflexivity.
+Grab Existential Variables.
+auto.
+Qed. 
+
+Fact merge_bs_length: forall l' l,
+length l = length l' ->
+length (merge_bs l l') = length l'.
+Proof.
+unfold merge_bs.
+induction l'; intros.
+apply length_zero_iff_nil in H; rewrite H.
+reflexivity.
+destruct l.
+simpl in H; inversion H.
+simpl; rewrite IHl'.
+reflexivity.
+simpl in H; omega.
+Qed.
+
+Fact updN_list_length: forall l a ln,
+a + length ln <= length l ->
+length (updN_list l a ln) = length l.
+Proof.
+intros.
+unfold updN_list.
+repeat rewrite app_length.
+rewrite merge_bs_length.
+rewrite firstn_length_l; try omega.
+rewrite skipn_length.
+rewrite Nat.add_assoc.
+symmetry; apply le_plus_minus.
+auto.
+apply get_sublist_length.
+auto.
+Qed.
+
+Fact updN_list2firstn_skipn: forall ln a l,
+a + length ln <= length l ->
+updN_list l a ln = firstn a l ++ (updN_list (get_sublist l a (length ln)) 0 ln) 
+                      ++ skipn (a + (length ln)) l.
+Proof.
+intros.
+unfold updN_list; simpl.
+unfold get_sublist; simpl.
+rewrite firstn_firstn.
+rewrite Nat.min_id.
+replace (firstn (length ln) (skipn a l)) with (firstn (length ln + 0) (skipn a l)).
+rewrite skipn_firstn_comm.
+simpl. rewrite app_nil_r. reflexivity.
+rewrite <- plus_n_O; reflexivity.
+Qed.
+
+Lemma bsplit_list_b2vb: forall b,
+exists l, (bsplit_list (bytes2valubytes (byte2bytes b))) = b::l.
+Proof. Admitted.
+
+
+
+(* Lemma byte_sep: forall a sz (b: bytes sz),
+natToWord ((sz + a) * 8) (#(b) * (Nat.pow 2 (a * 8))) = bcombine b (word2bytes a eq_refl (natToWord (a*8) 0)).
+intros.
+simpl.
+unfold natToWord, bcombine.
+eq_rect_simpl.
+destruct (eq_sym (Nat.mul_add_distr_r sz a 8)).
+eq_rect_simpl.
+induction (a * 8).
+simpl.
+rewrite Nat.mul_1_r.
+
+rewrite combine_n_0.
+rewrite <- plus_n_O.
+simpl.
+apply natToWord_wordToNat.
+simpl.
+Locate "~".
+unfold Word.combine in *.
+Admitted.
+
+
+Lemma byte1_split: forall a sz (b: bytes sz),
+  sz > 0 ->
+  bsplit_list (natToWord ((sz + a) * 8) (#(b) * (Nat.pow 2 (a * 8)))) =
+     (bsplit_list b) ++ (bsplit_list (natToWord (a * 8) (Nat.pow 2 (a*8)))).
+Proof.
+induction a; intros.
+simpl.
+unfold natToWord.
+rewrite <- plus_n_O.
+rewrite Nat.mul_1_r.
+rewrite natToWord_wordToNat.
+symmetry; apply app_nil_r.
+simpl.
+eq_rect_simpl.
+repeat rewrite <- plus_n_O.
+unfold bsplit1_dep, bsplit2_dep; simpl.
+replace (2 ^ (a * 8) + 2 ^ (a * 8) + (2 ^ (a * 8) + 2 ^ (a * 8))) with (4 * 2 ^ a). by omega.
+unfold wordToNat.
+simpl.
+unfold natToWord.
+replace (bsplit2 1 a $ (2 * 2 ^ a)) with (natToWord (a*8) 0).
+rewrite <- IHsz; auto.
+destruct sz.
+simpl.
+rewrite Nat.mul_assoc.
+unfold wordToNat.
+replace  ((fix wordToNat (sz0 : addr) (w : word sz0) {struct w} : addr :=
+      match w with
+      | WO => 0
+      | @WS true n w' => S (wordToNat n w' * 2)
+      | @WS false n w' => wordToNat n w' * 2
+      end) (S (S (S (S (S (S (S (S (sz * 8))))))))) b * 2 * 2 ^ a) with (2 * ((fix wordToNat (sz0 : addr) (w : word sz0) {struct w} : addr :=
+      match w with
+      | WO => 0
+      | @WS true n w' => S (wordToNat n w' * 2)
+      | @WS false n w' => wordToNat n w' * 2
+      end) (S (S (S (S (S (S (S (S (sz * 8))))))))) b * 2 ^ a)).
+unfold natToWord.
+repeat rewrite div2_double.
+fold wordToNat.
+rewrite <- IHa.
+simpl.
+ bsplit_list.
+simpl.
+ *)
+
+
 (*Specs*)
+Theorem dwrite_to_block_ok : forall lxp bxp ixp inum block_off byte_off data fms,
+    {< F Fm Fi Fd ds flist ilist frees f fy old_data p1 p2,
+    PRE:hm
+           LOG.rep lxp F (LOG.ActiveTxn ds ds!!) (BFILE.MSLL fms) hm *
+           [[[ ds!! ::: (Fm * BFILE.rep bxp ixp flist ilist frees) ]]] *
+           [[[ flist ::: (Fi * inum |-> f) ]]] *
+           rep f fy  *
+           [[[ (ByFData fy) ::: (Fd * arrayN (ptsto (V:=byteset)) (block_off * valubytes) (p1 ++ old_data ++ p2))]]] *
+           [[ length old_data = length data]] *
+           [[ length old_data > 0 ]] *
+           [[ byte_off + length data <= valubytes ]] *
+           [[ length p1 = byte_off ]] *
+           [[ length (p1++old_data++p2) = valubytes ]] *
+           [[ sync_invariant F ]]
+     POST:hm' RET:fms'  exists flist' f' bn ds0 ds',
+           let fy' := mk_bytefile (updN_list (ByFData fy) 
+              (block_off * valubytes) 
+              ((map fst p1)++data++(map fst p2))) (ByFAttr fy) in  
+           LOG.rep lxp F (LOG.ActiveTxn ds' ds'!!) (BFILE.MSLL fms') hm' *
+           [[ ds' = dsupd ds0 bn 
+                ((list2valu ((map fst p1)++data++(map fst p2))), 
+                vsmerge (selN (BFILE.BFData f) block_off valuset0)) 
+              /\ BFILE.diskset_was ds0 ds ]] *
+           [[ BFILE.block_belong_to_file ilist bn inum block_off ]] *
+           [[[ ds'!! ::: (Fm  * BFILE.rep bxp ixp flist' ilist frees) ]]] *
+           [[[ flist' ::: (Fi * inum |-> f') ]]] *
+           rep f' fy' *
+           [[[ (ByFData fy') ::: (Fd * arrayN (ptsto (V:=byteset)) 
+           (block_off * valubytes) (updN_list (p1++old_data++p2) 0 
+                    ((map fst p1)++data++(map fst p2))))]]] *
+           [[ BFILE.MSAlloc fms = BFILE.MSAlloc fms' ]]
+    XCRASH:hm'
+          LOG.recover_any lxp F ds hm' \/
+          exists bn, [[ BFILE.block_belong_to_file ilist bn inum block_off ]] *
+           LOG.recover_any lxp F (dsupd ds bn ((list2valu ((map fst p1)++data++(map fst p2))), 
+                vsmerge (selN (BFILE.BFData f) block_off valuset0))) hm'
+    >} dwrite_to_block lxp ixp inum fms block_off byte_off data.
+
+Proof.
+unfold dwrite_to_block, rep.
+step.
+
+eapply inlen_bfile; try eauto; try omega.
+instantiate (1:= length p1); rewrite valubytes_is in *; omega.
+repeat rewrite arrayN_app in H11.
+pred_apply.
+cancel.
+
+instantiate (1:= (selN (BFILE.BFData f) block_off valuset0)).
+instantiate (1:= diskIs(mem_except (list2nmem (BFILE.BFData f)) block_off )).
+apply addr_id.
+
+eapply inlen_bfile; try eauto; try omega.
+instantiate (1:= length p1); rewrite valubytes_is in *; omega.
+repeat rewrite arrayN_app in H11.
+pred_apply.
+cancel.
+
+safestep.
+
+eapply inlen_bfile; try eauto; try omega.
+instantiate (1:= length p1); rewrite valubytes_is in *; omega.
+repeat rewrite arrayN_app in H11.
+pred_apply.
+cancel.
+
+instantiate (1:= (selN (BFILE.BFData f) block_off valuset0)).
+instantiate (1:= diskIs(mem_except (list2nmem (BFILE.BFData f)) block_off )).
+apply addr_id.
+
+eapply inlen_bfile; try eauto; try omega.
+instantiate (1:= length p1); rewrite valubytes_is in *; omega.
+repeat rewrite arrayN_app in H11.
+pred_apply.
+cancel.
+
+safestep.
+
+simpl.
+
+replace (firstn (length p1) (valu2list (fst (BFILE.BFData f) ⟦ block_off ⟧))) with 
+(map fst p1).
+
+replace (skipn (length p1 + length data) (valu2list (fst (BFILE.BFData f) ⟦ block_off ⟧))) with (map fst p2).
+reflexivity.
+
+apply arrayN_list2nmem in H11 as H'.
+rewrite H21 in H'; rewrite H22 in H'; rewrite H12 in H'.
+rewrite <- skipn_firstn_comm in H'.
+rewrite firstn_firstn in H'.
+rewrite Nat.min_l in H'.
+rewrite skipn_firstn_comm in H'.
+rewrite concat_hom_skipn in H'.
+rewrite H6 in H'.
+rewrite skipn_map_comm in H'.
+replace (valubytes) with (1*valubytes) in H' by omega.
+rewrite concat_hom_firstn in H'.
+rewrite firstn1 in H'.
+erewrite selN_map in H'.
+erewrite skipn_selN in H'.
+rewrite <- plus_n_O in H'.
+unfold valuset2bytesets in H'.
+unfold byteset2list in H'.
+simpl in H'.
+
+apply map_same with (f:= fst) in H'.
+rewrite mapfst_valuset2bytesets in H'.
+rewrite <- H'.
+repeat rewrite map_app.
+rewrite <- H10.
+repeat rewrite <- map_length with (f:= fst).
+rewrite skipn_app_r.
+rewrite skipn_app.
+reflexivity.
+
+rewrite Forall_forall; intros.
+destruct H7.
+rewrite <- H7; apply valu2list_len.
+apply in_map_iff in H7.
+repeat destruct H7.
+apply valu2list_len.
+rewrite skipn_length.
+apply Nat.lt_add_lt_sub_r.
+simpl.
+
+eapply inlen_bfile; try eauto; try omega.
+instantiate (1:= length p1); rewrite valubytes_is in *; omega.
+repeat rewrite arrayN_app in H11.
+pred_apply.
+cancel.
+
+rewrite Forall_forall; intros.
+apply in_map_iff in H7.
+repeat destruct H7.
+apply valuset2bytesets_len.
+
+rewrite Forall_forall; intros.
+apply in_map_iff in H7.
+repeat destruct H7.
+apply valuset2bytesets_len.
+
+apply list2nmem_arrayN_bound in H11 as H0'.
+destruct H0'.
+apply app_eq_nil in H7.
+destruct H7.
+apply app_eq_nil in H14.
+destruct H14.
+apply length_zero_iff_nil in H14.
+rewrite valubytes_is in *; omega.
+auto.
+apply byteset0.
+
+
+apply arrayN_list2nmem in H11 as H'.
+rewrite H21 in H'; rewrite H22 in H'; rewrite H12 in H'.
+rewrite <- skipn_firstn_comm in H'.
+rewrite firstn_firstn in H'.
+rewrite Nat.min_l in H'.
+rewrite skipn_firstn_comm in H'.
+rewrite concat_hom_skipn in H'.
+rewrite H6 in H'.
+rewrite skipn_map_comm in H'.
+replace (valubytes) with (1*valubytes) in H' by omega.
+rewrite concat_hom_firstn in H'.
+rewrite firstn1 in H'.
+erewrite selN_map in H'.
+erewrite skipn_selN in H'.
+rewrite <- plus_n_O in H'.
+unfold valuset2bytesets in H'.
+unfold byteset2list in H'.
+simpl in H'.
+
+apply map_same with (f:= fst) in H'.
+rewrite mapfst_valuset2bytesets in H'.
+rewrite <- H'.
+repeat rewrite map_app.
+repeat rewrite <- map_length with (f:= fst).
+rewrite firstn_app_l.
+rewrite firstn_oob.
+reflexivity.
+omega.
+omega.
+
+
+
+rewrite Forall_forall; intros.
+destruct H7.
+rewrite <- H7; apply valu2list_len.
+apply in_map_iff in H7.
+repeat destruct H7.
+apply valu2list_len.
+rewrite skipn_length.
+apply Nat.lt_add_lt_sub_r.
+simpl.
+
+eapply inlen_bfile; try eauto; try omega.
+instantiate (1:= length p1); rewrite valubytes_is in *; omega.
+repeat rewrite arrayN_app in H11.
+pred_apply.
+cancel.
+
+rewrite Forall_forall; intros.
+apply in_map_iff in H7.
+repeat destruct H7.
+apply valuset2bytesets_len.
+
+rewrite Forall_forall; intros.
+apply in_map_iff in H7.
+repeat destruct H7.
+apply valuset2bytesets_len.
+
+apply list2nmem_arrayN_bound in H11 as H0'.
+destruct H0'.
+apply app_eq_nil in H7.
+destruct H7.
+apply app_eq_nil in H14.
+destruct H14.
+apply length_zero_iff_nil in H14.
+rewrite valubytes_is in *; omega.
+auto.
+apply byteset0.
+
+auto.
+auto.
+
+instantiate (1:= mk_proto_bytefile (updN (PByFData pfy) block_off (valuset2bytesets(list2valu
+                        (firstn (length p1) (valu2list (fst (selN (BFILE.BFData f) block_off valuset0))) ++
+                         data ++ skipn (length p1 + length data) (valu2list (fst (selN (BFILE.BFData f) block_off valuset0)))),
+                     vsmerge (selN (BFILE.BFData f) block_off valuset0))))).
+unfold proto_bytefile_valid; simpl.
+rewrite H12.
+rewrite map_updN.
+apply updN_eq.
+reflexivity.
+
+instantiate (1:= (mk_unified_bytefile (firstn (block_off * valubytes) (UByFData ufy) ++ (valuset2bytesets
+                   (list2valu
+                      (firstn (length p1) (valu2list (fst (BFILE.BFData f) ⟦ block_off ⟧)) ++
+                       data ++ skipn (length p1 + length data) (valu2list (fst (BFILE.BFData f) ⟦ block_off ⟧))),
+                   vsmerge (BFILE.BFData f) ⟦ block_off ⟧)) ++
+        skipn (block_off * valubytes + valubytes) (UByFData ufy)))).
+unfold unified_bytefile_valid.
+simpl.
+rewrite H22.
+rewrite <- concat_hom_updN_first_skip with (k:= valubytes).
+reflexivity.
+
+eapply proto_len; eauto.
+
+erewrite bfile_protobyte_len_eq; eauto.
+eapply inlen_bfile; try eauto; try omega.
+instantiate (1:= length p1); rewrite valubytes_is in *; omega.
+repeat rewrite arrayN_app in H11.
+pred_apply.
+cancel.
+
+Focus 2.
+rewrite updN_list_length; auto.
+
+Focus 3.
+cancel.
+repeat xcrash_rewrite.
+xform_norm; xform_normr.
+cancel.
+
+or_r; cancel.
+
+apply arrayN_list2nmem in H11 as H'.
+rewrite H21 in H'; rewrite H22 in H'; rewrite H12 in H'.
+rewrite <- skipn_firstn_comm in H'.
+rewrite firstn_firstn in H'.
+rewrite Nat.min_l in H'.
+rewrite skipn_firstn_comm in H'.
+rewrite concat_hom_skipn in H'.
+rewrite H6 in H'.
+rewrite skipn_map_comm in H'.
+replace (valubytes) with (1*valubytes) in H' by omega.
+rewrite concat_hom_firstn in H'.
+rewrite firstn1 in H'.
+erewrite selN_map in H'.
+erewrite skipn_selN in H'.
+rewrite <- plus_n_O in H'.
+unfold valuset2bytesets in H'.
+unfold byteset2list in H'.
+simpl in H'.
+
+apply map_same with (f:= fst) in H'.
+rewrite mapfst_valuset2bytesets in H'.
+rewrite <- H'.
+repeat rewrite map_app.
+repeat rewrite <- map_length with (f:= fst).
+rewrite firstn_app_l.
+rewrite firstn_oob.
+rewrite <- H10.
+rewrite skipn_app_r.
+replace (length old_data) with (length (map fst old_data) + 0).
+rewrite skipn_app_r; simpl.
+instantiate (1:= x).
+xform_norm; cancel.
+rewrite map_length; omega.
+omega.
+omega.
+rewrite Forall_forall; intros.
+repeat destruct H7.
+apply valu2list_len.
+apply in_map_iff in H7.
+repeat destruct H7.
+apply valu2list_len.
+
+rewrite skipn_length.
+apply Nat.lt_add_lt_sub_r.
+simpl; eapply inlen_bfile; try eauto; try omega.
+instantiate (1:= length p1); rewrite valubytes_is in *; omega.
+repeat rewrite arrayN_app in H11.
+pred_apply.
+cancel.
+rewrite <- skipn_map_comm.
+rewrite <- H12.
+eapply proto_skip_len; eauto.
+rewrite <- H12.
+eapply proto_len; eauto.
+
+apply list2nmem_arrayN_bound in H11 as H0'.
+destruct H0'.
+rewrite app_assoc in H7.
+apply app_eq_nil in H7.
+destruct H7.
+apply app_eq_nil in H7.
+destruct H7.
+rewrite H17 in H9.
+inversion H9.
+auto.
+apply byteset0.
+
+Focus 3.
+cancel.
+
+xcrash.
+or_l; rewrite LOG.active_intact, LOG.intact_any; auto.
+
+
+Focus 2.
+apply arrayN_list2nmem in H11 as H'.
+rewrite updN_list2firstn_skipn with (a:= block_off*valubytes).
+unfold get_sublist.
+replace (length (map fst p1 ++ data ++ map fst p2)) with (length (p1 ++ old_data ++ p2)).
+rewrite <- H'.
+
+replace (arrayN (ptsto (V:=byteset)) (block_off * valubytes) (updN_list (p1 ++ old_data ++ p2) 0 (map fst p1 ++ data ++ map fst p2)))
+
+with (arrayN (ptsto (V:=byteset)) (length (firstn (block_off * valubytes) (ByFData fy))) (updN_list (p1 ++ old_data ++ p2) 0 (map fst p1 ++ data ++ map fst p2))).
+
+apply list2nmem_arrayN_middle.
+
+apply arrayN_frame_mem_ex_range in H11 as H0'.
+rewrite firstn_length_l. rewrite updN_list_length.
+
+replace (mem_except_range
+     (list2nmem
+        (firstn (block_off * valubytes) (ByFData fy) ++
+         updN_list (p1 ++ old_data ++ p2) 0 (map fst p1 ++ data ++ map fst p2) ++
+         skipn (block_off * valubytes + length (p1 ++ old_data ++ p2)) (ByFData fy))) (block_off * valubytes)
+     (length (p1 ++ old_data ++ p2)))
+     
+     with (mem_except_range (list2nmem (ByFData fy)) (block_off * valubytes) (length (p1 ++ old_data ++ p2))). auto.
+
+apply functional_extensionality; intros.
+unfold mem_except_range.
+
+destruct (le_dec (block_off * valubytes) x);
+destruct (lt_dec x (block_off * valubytes + length (p1 ++ old_data ++ p2)));
+destruct (lt_dec x (length (ByFData fy)));
+try omega; try reflexivity.
+
+unfold list2nmem.
+repeat erewrite selN_map.
+rewrite selN_app2.
+rewrite selN_app2.
+rewrite skipn_selN.
+rewrite firstn_length_l.
+rewrite updN_list_length.
+replace (block_off * valubytes + length (p1 ++ old_data ++ p2) + (x - block_off * valubytes - length (p1 ++ old_data ++ p2))) with x.
+reflexivity.
+replace((x - block_off * valubytes - length (p1 ++ old_data ++ p2))) with 
+((x - (block_off * valubytes + length (p1 ++ old_data ++ p2)))) by omega.
+apply le_plus_minus.
+omega.
+
+apply list2nmem_arrayN_bound in H11 as H1'.
+destruct H1'.
+rewrite app_assoc in H7.
+apply app_eq_nil in H7.
+destruct H7.
+apply app_eq_nil in H7.
+destruct H7.
+rewrite H15 in H9.
+inversion H9.
+omega.
+
+rewrite firstn_length_l.
+rewrite updN_list_length.
+omega.
+
+
+apply list2nmem_arrayN_bound in H11 as H1'.
+destruct H1'.
+rewrite app_assoc in H7.
+apply app_eq_nil in H7.
+destruct H7.
+apply app_eq_nil in H7.
+destruct H7.
+rewrite H15 in H9.
+inversion H9.
+omega.
+
+rewrite firstn_length_l.
+omega.
+
+apply list2nmem_arrayN_bound in H11 as H1'.
+destruct H1'.
+rewrite app_assoc in H7.
+apply app_eq_nil in H7.
+destruct H7.
+apply app_eq_nil in H7.
+destruct H7.
+rewrite H15 in H9.
+inversion H9.
+omega.
+
+repeat rewrite app_length.
+rewrite firstn_length_l.
+rewrite updN_list_length.
+rewrite skipn_length.
+repeat rewrite app_length. omega.
+
+apply list2nmem_arrayN_bound in H11 as H1'.
+destruct H1'.
+rewrite app_assoc in H7.
+apply app_eq_nil in H7.
+destruct H7.
+apply app_eq_nil in H7.
+destruct H7.
+rewrite H15 in H9.
+inversion H9.
+omega.
+
+auto.
+
+repeat rewrite list2nmem_oob.
+reflexivity.
+
+repeat rewrite app_length.
+rewrite firstn_length_l.
+rewrite updN_list_length.
+rewrite skipn_length.
+repeat rewrite app_length.
+remember (block_off * valubytes + (length p1 + (length old_data + length p2))) as c.
+rewrite Nat.add_assoc.
+rewrite <- Heqc.
+rewrite <- le_plus_minus.
+omega.
+
+rewrite Heqc.
+apply list2nmem_arrayN_bound in H11 as H1'.
+destruct H1'.
+rewrite app_assoc in H7.
+apply app_eq_nil in H7.
+destruct H7.
+apply app_eq_nil in H7.
+destruct H7.
+rewrite H15 in H9.
+inversion H9.
+repeat rewrite app_length in H7.
+omega.
+
+apply list2nmem_arrayN_bound in H11 as H1'.
+destruct H1'.
+rewrite app_assoc in H7.
+apply app_eq_nil in H7.
+destruct H7.
+apply app_eq_nil in H7.
+destruct H7.
+rewrite H15 in H9.
+inversion H9.
+repeat rewrite app_length in H7.
+omega.
+
+omega.
+
+
+
+unfold list2nmem.
+repeat erewrite selN_map.
+rewrite selN_app1.
+rewrite selN_firstn.
+reflexivity.
+omega.
+rewrite firstn_length_l.
+omega.
+
+apply list2nmem_arrayN_bound in H11 as H1'.
+destruct H1'.
+rewrite app_assoc in H7.
+apply app_eq_nil in H7.
+destruct H7.
+apply app_eq_nil in H7.
+destruct H7.
+rewrite H15 in H9.
+inversion H9.
+repeat rewrite app_length in H7.
+omega.
+
+
+repeat rewrite app_length.
+rewrite firstn_length_l.
+rewrite updN_list_length.
+rewrite skipn_length.
+repeat rewrite app_length. omega.
+
+apply list2nmem_arrayN_bound in H11 as H1'.
+destruct H1'.
+rewrite app_assoc in H7.
+apply app_eq_nil in H7.
+destruct H7.
+apply app_eq_nil in H7.
+destruct H7.
+rewrite H15 in H9.
+inversion H9.
+omega.
+
+auto.
+
+repeat rewrite list2nmem_oob.
+reflexivity.
+
+repeat rewrite app_length.
+rewrite firstn_length_l.
+rewrite updN_list_length.
+rewrite skipn_length.
+repeat rewrite app_length.
+remember (block_off * valubytes + (length p1 + (length old_data + length p2))) as c.
+rewrite Nat.add_assoc.
+rewrite <- Heqc.
+rewrite <- le_plus_minus.
+omega.
+
+rewrite Heqc.
+apply list2nmem_arrayN_bound in H11 as H1'.
+destruct H1'.
+rewrite app_assoc in H7.
+apply app_eq_nil in H7.
+destruct H7.
+apply app_eq_nil in H7.
+destruct H7.
+rewrite H15 in H9.
+inversion H9.
+repeat rewrite app_length in H7.
+omega.
+
+apply list2nmem_arrayN_bound in H11 as H1'.
+destruct H1'.
+rewrite app_assoc in H7.
+apply app_eq_nil in H7.
+destruct H7.
+apply app_eq_nil in H7.
+destruct H7.
+rewrite H15 in H9.
+inversion H9.
+repeat rewrite app_length in H7.
+omega.
+
+omega.
+
+apply list2nmem_arrayN_bound in H11 as H1'.
+destruct H1'.
+rewrite app_assoc in H7.
+apply app_eq_nil in H7.
+destruct H7.
+apply app_eq_nil in H7.
+destruct H7.
+rewrite H15 in H9.
+inversion H9.
+repeat rewrite app_length in H7.
+omega.
+
+rewrite firstn_length_l. reflexivity.
+
+apply list2nmem_arrayN_bound in H11 as H1'.
+destruct H1'.
+rewrite app_assoc in H7.
+apply app_eq_nil in H7.
+destruct H7.
+apply app_eq_nil in H7.
+destruct H7.
+rewrite H15 in H9.
+inversion H9.
+repeat rewrite app_length in H7.
+omega.
+
+repeat rewrite app_length.
+repeat rewrite map_length.
+omega.
+
+repeat rewrite app_length.
+repeat rewrite map_length.
+apply list2nmem_arrayN_bound in H11 as H1'.
+destruct H1'.
+rewrite app_assoc in H7.
+apply app_eq_nil in H7.
+destruct H7.
+apply app_eq_nil in H7.
+destruct H7.
+rewrite H15 in H9.
+inversion H9.
+repeat rewrite app_length in H7.
+omega.
+
+apply byteset0.
+
+
+unfold bytefile_valid; simpl.
+rewrite updN_list_length.
+
+replace (length (ByFData fy)) with
+
+(length (firstn (block_off * valubytes) (UByFData ufy)) +
+   (length (valuset2bytesets
+     (list2valu
+        (firstn (length p1) (valu2list (fst (selN (BFILE.BFData f) block_off valuset0))) ++
+         data ++ skipn (length p1 + length data) (valu2list (fst (selN (BFILE.BFData f) block_off valuset0)))),
+     vsmerge (selN (BFILE.BFData f) block_off valuset0))) + (length (ByFData fy) - (length (firstn (block_off * valubytes) (UByFData ufy)) +
+   length (valuset2bytesets
+     (list2valu
+        (firstn (length p1) (valu2list (fst (selN (BFILE.BFData f) block_off valuset0))) ++
+         data ++ skipn (length p1 + length data) (valu2list (fst (selN (BFILE.BFData f) block_off valuset0)))),
+     vsmerge (selN (BFILE.BFData f) block_off valuset0))))))).
+repeat rewrite firstn_app_r.
+
+rewrite <- skipn_firstn_comm.
+rewrite firstn_length_l.
+rewrite valuset2bytesets_len.
+
+replace ((block_off * valubytes + valubytes + (length (ByFData fy) - (block_off * valubytes + valubytes)))) with (length (ByFData fy)).
+
+rewrite updN_list2firstn_skipn.
+repeat rewrite app_length in *.
+repeat rewrite map_length.
+rewrite H10 in H6.
+rewrite H6.
+
+rewrite H21.
+rewrite firstn_firstn.
+rewrite Nat.min_l.
+unfold get_sublist.
+rewrite <- skipn_firstn_comm.
+rewrite firstn_firstn.
+rewrite Nat.min_l.
+
+rewrite firstn_length_l.
+
+replace (updN_list (skipn (block_off * valubytes) (firstn (block_off * valubytes + valubytes) (UByFData ufy))) 0
+  (map fst p1 ++ data ++ map fst p2))
+  
+  with (valuset2bytesets
+  (list2valu
+     (firstn (length p1) (valu2list (fst (selN (BFILE.BFData f) block_off valuset0))) ++
+      data ++ skipn (length p1 + length data) (valu2list (fst (selN (BFILE.BFData f) block_off valuset0)))), vsmerge (selN (BFILE.BFData f) block_off valuset0))).
+      reflexivity.
+      
+unfold valuset2bytesets.
+unfold byteset2list.
+simpl.
+rewrite list2valu2list.
+
+rewrite H22; rewrite H12.
+rewrite skipn_firstn_comm.
+rewrite concat_hom_skipn.
+replace (valubytes) with (1 * valubytes) by omega.
+rewrite concat_hom_firstn.
+rewrite firstn1.
+rewrite skipn_selN.
+rewrite selN_map with (default' := valuset0).
+simpl.
+repeat rewrite <- plus_n_O.
+unfold valuset2bytesets.
+unfold byteset2list.
+simpl.
+
+Admitted.
+
+
+
+Hint Extern 1 ({{_}} Bind (dwrite_to_block _ _ _ _ _ _ _) _) => apply write_to_block_ok : prog.
+
+
+
 
 Theorem write_to_block_ok : forall lxp bxp ixp inum block_off byte_off data fms,
     {< F Fm Fi Fd flist ilist frees m0 m f fy old_data,
@@ -1511,6 +2365,168 @@ apply byteset0.
 apply byteset0.
 Qed.
 
+Hint Extern 1 ({{_}} Bind (write_to_block _ _ _ _ _ _ _) _) => apply write_to_block_ok : prog.
+
+Theorem getlen_ok : forall lxp bxp ixp inum fms,
+{< F Fm Fi m0 m flist ilist frees f fy,
+PRE:hm
+       LOG.rep lxp F (LOG.ActiveTxn m0 m) (BFILE.MSLL fms) hm *
+       [[[ m ::: (Fm * BFILE.rep bxp ixp flist ilist frees) ]]] *
+       [[[ flist ::: (Fi * inum |-> f) ]]] *
+       rep f fy
+POST:hm' RET:^(fms',r)
+       LOG.rep lxp F (LOG.ActiveTxn m0 m) (BFILE.MSLL fms') hm' *
+       [[ r = length (ByFData fy)]] *
+       [[ BFILE.MSAlloc fms = BFILE.MSAlloc fms' ]]
+CRASH:hm'  exists fms',
+       LOG.rep lxp F (LOG.ActiveTxn m0 m) (BFILE.MSLL fms') hm'
+>} getlen lxp ixp inum fms.
+Proof.
+unfold getlen, rep.
+hoare.
+Qed.
+
+Hint Extern 1 ({{_}} Bind (getlen _ _ _ _) _) => apply getlen_ok : prog.
+
+Theorem grow_ok : forall lxp bxp ixp inum b ms,
+    {< F Fm Fi Fd  m0 m flist ilist frees f fy,
+    PRE:hm
+           LOG.rep lxp F (LOG.ActiveTxn m0 m) (BFILE.MSLL ms) hm *
+           [[[ m ::: (Fm * BFILE.rep bxp ixp flist ilist frees) ]]] *
+           [[[ flist ::: (Fi * inum |-> f) ]]] *
+           rep f fy  *
+           [[[ (ByFData fy) ::: Fd]]] 
+    POST:hm' RET:^(ms', r) [[ BFILE.MSAlloc ms = BFILE.MSAlloc ms' ]] * exists m',
+           let fy' := mk_bytefile ((ByFData fy) ++ ((b,nil)::nil))%list ($ (S (length (ByFData fy))), snd (ByFAttr fy)) in
+           [[ r = false ]] * LOG.rep lxp F (LOG.ActiveTxn m0 m') (BFILE.MSLL ms') hm' \/
+           [[ r = true  ]] * exists flist' ilist' frees' f',
+           LOG.rep lxp F (LOG.ActiveTxn m0 m') (BFILE.MSLL ms') hm' *
+           [[[ m' ::: (Fm * BFILE.rep bxp ixp flist' ilist' frees') ]]] *
+           [[[ flist' ::: (Fi * inum |-> f') ]]] *
+           rep f' fy'  *
+           [[[ (ByFData fy') ::: (Fd * (length (ByFData fy)) |-> (b, nil))]]] *
+           [[ ByFAttr fy' = ($ (S (length (ByFData fy))), snd (ByFAttr fy)) ]] *
+           [[ BFILE.ilist_safe ilist  (BFILE.pick_balloc frees  (BFILE.MSAlloc ms'))
+                         ilist' (BFILE.pick_balloc frees' (BFILE.MSAlloc ms')) ]]
+    CRASH:hm'  LOG.intact lxp F m0 hm'
+    >} grow lxp bxp ixp inum b ms.
+Proof.
+unfold grow, rep.
+prestep.
+norm.
+unfold stars; cancel.
+unfold rep; cancel; eauto.
+intuition; eauto.
+step.
+step.
+step.
+instantiate (1:= diskIs (list2nmem (BFILE.BFData f)) ); apply diskIs_id.
+step.
+step.
+step.
+step.
+step.
+right.
+pred_apply.
+cancel.
+instantiate (1:= mk_proto_bytefile ((PByFData pfy) ++ (valuset2bytesets (byte2valu b, nil))::nil)).
+unfold proto_bytefile_valid; simpl.
+rewrite map_app.
+simpl.
+rewrite H6; reflexivity.
+instantiate (1:= mk_unified_bytefile ((UByFData ufy) ++ (valuset2bytesets (byte2valu b, nil)))).
+unfold unified_bytefile_valid; simpl.
+rewrite concat_app; simpl.
+rewrite app_nil_r.
+rewrite H16; reflexivity.
+unfold bytefile_valid; simpl.
+rewrite app_length; simpl.
+rewrite H15; simpl.
+rewrite firstn_length_l.
+rewrite H18.
+
+erewrite <- bfile_protobyte_len_eq; eauto.
+erewrite <- unified_byte_protobyte_len; eauto.
+rewrite firstn_app_r.
+rewrite firstn_oob; try omega.
+unfold byte2valu.
+unfold valuset2bytesets.
+unfold byteset2list.
+simpl.
+rewrite v2b_rec_nil.
+unfold cons'.
+rewrite map_map; simpl.
+unfold valu2list.
+rewrite bytes2valu2bytes.
+
+Focus 2.
+rewrite valu2list_len; reflexivity.
+
+Focus 2.
+eapply proto_len; eauto.
+
+Focus 2.
+eapply bytefile_unified_byte_len; eauto.
+
+Focus 2.
+rewrite H14; reflexivity.
+
+Focus 3.
+apply list2nmem_app; auto.
+
+Focus 3.
+eapply BFILE.ilist_safe_trans; eauto.
+rewrite <- H34; auto.
+
+Focus 3.
+step.
+
+Focus 3.
+step.
+
+pose proof bsplit_list_b2vb.
+destruct H20 with (b:=b).
+rewrite H23.
+simpl.
+reflexivity.
+
+
+eapply bytefile_unified_byte_len; eauto.
+rewrite H14; reflexivity.
+rewrite app_length; simpl.
+unfold wordToNat.
+unfold natToWord.
+pose proof wordToNat_natToWord.
+
+
+
+unfold bytes2valubytes.
+simpl.
+unfold byte in b.
+destruct (le_dec 1 valubytes).
+unfold bcombine.
+eq_rect_simpl.
+unfold bsplit_list. simpl.
+rewrite valubytes_is; simpl.
+simpl.
+
+inversion H0.
+contradiction.
+unfold bytes2valubytes.
+simpl.
+unfold natToWord.
+rewrite valubytes_is.
+simpl.
+destruct (bsplit_list $ (# (b) * 2 ^ (valubytes - 1))) eqn:D.
+apply length_zero_iff_nil in D.
+rewrite bsplit_list_len in D.
+rewrite valubytes_is in D; inversion D.
+simpl in *.
+Admitted.
+
+Hint Extern 1 ({{_}} Bind (grow _ _ _ _ _ _) _) => apply grow_ok : prog.
+
+
 
 Theorem write_middle_blocks_ok : forall lxp bxp ixp inum block_off num_of_full_blocks data fms,
     {< F Fm Fi Fd m0 m flist ilist frees f fy old_data,
@@ -1539,23 +2555,46 @@ Theorem write_middle_blocks_ok : forall lxp bxp ixp inum block_off num_of_full_b
     >} write_middle_blocks lxp ixp inum fms block_off num_of_full_blocks data.
 Proof.
 unfold write_middle_blocks, rep.
-step.
-
-apply emp_star_r.
+safestep.
+rewrite <- plus_n_O.
+apply list2nmem_arrayN_bound in H9 as H'.
+destruct H'.
+apply length_zero_iff_nil in H.
+rewrite valubytes_is in *; omega.
+rewrite H7 in H; rewrite H5 in H.
+instantiate (1:= fy).
+rewrite valubytes_is in *; omega.
 eauto.
+eauto.
+eauto.
+eauto.
+eauto.
+instantiate (1:= diskIs (list2nmem (BFILE.BFData f)) ).
+apply emp_star_r; apply diskIs_id.
+apply emp_star_r; eauto.
+apply H8; auto.
+exists nil; constructor.
 
 monad_simpl.
 eapply pimpl_ok2.
 apply write_to_block_ok.
 
 intros; norm.
-unfold stars, rep; cancel.
-instantiate (1:= mk_proto_bytefile (updN (PByFData pfy) (block_off + m1) 
+unfold stars; cancel.
+
+instantiate (2:= BFILE.mk_bfile (updN (BFILE.BFData f0) (block_off + m1) 
+                                      (list2valu (get_sublist data (m1 * valubytes) valubytes), nil))
+ (BFILE.BFAttr f0)).
+
+instantiate (1:= mk_bytefile (firstn ((block_off + m1) * valubytes) (ByFData fy0) ++
+              map (fun x : byte => (x, nil)) (get_sublist data (m1 * valubytes) valubytes) ++
+              skipn ((block_off + m1) * valubytes + valubytes) (ByFData fy0)) (ByFAttr fy0)).
+unfold rep; cancel.
+
+instantiate (1:= mk_proto_bytefile (updN (PByFData pfy0) (block_off + m1) 
                                       (map (fun x => (x,nil)) (get_sublist data (m1 * valubytes) valubytes)))).
-instantiate (1:= BFILE.mk_bfile (updN (BFILE.BFData f) (block_off + m1) 
-                                      (list2valu (get_sublist data (m1 * valubytes) valubytes), nil)) (BFILE.BFAttr f)).
 unfold proto_bytefile_valid; simpl.
-rewrite H10.
+rewrite H24.
 rewrite map_updN.
 unfold valuset2bytesets.
 unfold byteset2list.
@@ -1565,40 +2604,31 @@ rewrite v2b_rec_nil.
 unfold cons'.
 rewrite map_map; reflexivity.
 
-unfold get_sublist.
-rewrite firstn_length.
-rewrite Nat.min_l.
-reflexivity.
-rewrite skipn_length.
-rewrite H5.
-rewrite valubytes_is; omega.
+symmetry; apply get_sublist_length; eauto.
+rewrite valubytes_is in *; omega.
 
-unfold get_sublist.
-rewrite firstn_length.
-rewrite Nat.min_l.
-reflexivity.
-rewrite skipn_length.
-rewrite H5.
-rewrite valubytes_is; omega.
+apply get_sublist_length; eauto.
+rewrite valubytes_is in *; omega.
 
-instantiate (1:= mk_unified_bytefile (firstn ((block_off + m1) * valubytes) (UByFData ufy) ++ 
+instantiate (1:= mk_unified_bytefile (firstn ((block_off + m1) * valubytes) (UByFData ufy0) ++ 
                                       map (fun x => (x,nil)) (get_sublist data (m1 * valubytes) valubytes) ++
-                                      skipn ((block_off + m1) * valubytes + valubytes) (UByFData ufy))).
+                                      skipn ((block_off + m1) * valubytes + valubytes) (UByFData ufy0))).
 unfold unified_bytefile_valid; simpl.
-rewrite H20; simpl.
+rewrite H37; simpl.
 rewrite <- concat_hom_updN_first_skip with (k:= valubytes).
 reflexivity.
 eapply proto_len; eauto.
+apply le2lt_l in H25; eauto.
+eapply unibyte_len in H25; eauto.
+rewrite H37 in H25.
+rewrite concat_hom_length with (k:= valubytes) in H25.
+apply le_mult_weaken in H25; auto.
+rewrite valubytes_is; omega.
+eapply proto_len; eauto.
+rewrite valubytes_is; omega.
 
-eapply inbound_protobyte; eauto.
-rewrite H7; rewrite H5; apply mult_lt_compat_r; try rewrite valubytes_is; omega.
-
- 
-instantiate (1:= mk_bytefile (firstn ((block_off + m1) * valubytes) (ByFData fy) ++
-              map (fun x : byte => (x, nil)) (get_sublist data (m1 * valubytes) valubytes) ++
-              skipn ((block_off + m1) * valubytes + valubytes) (ByFData fy)) (ByFAttr fy)).
 unfold bytefile_valid; simpl.
-rewrite H19.
+rewrite H36.
 rewrite app_length.
 repeat rewrite firstn_firstn.
 rewrite Nat.min_l.
@@ -1608,34 +2638,17 @@ rewrite firstn_app_r.
 rewrite skipn_length.
 rewrite firstn_length_l.
 rewrite <- skipn_firstn_comm.
-replace  ((block_off + m1) * valubytes + valubytes + (length (ByFData fy) - ((block_off + m1) * valubytes + valubytes)))
-      with (length (ByFData fy)).
+replace  ((block_off + m1) * valubytes + valubytes + (length (ByFData fy0) - ((block_off + m1) * valubytes + valubytes)))
+      with (length (ByFData fy0)).
 reflexivity.
 
 remember ((block_off + m1) * valubytes + valubytes) as b.
 apply le_plus_minus.
-rewrite Heqb.
-apply list2nmem_arrayN_bound in H9 as H'.
-destruct H'.
-rewrite <- length_zero_iff_nil in H14. 
-rewrite H14 in H7; rewrite <- H7 in H5; rewrite valubytes_is in H5; omega.
-rewrite H7 in H14; rewrite H5 in H14.
-unfold lt in H.
-rewrite valubytes_is in *; omega.
+auto.
 
-apply bytefile_unified_byte_len; auto.
+eapply bytefile_unified_byte_len; eauto.
+omega.
 
-
-apply list2nmem_arrayN_bound in H9 as H'.
-destruct H'.
-rewrite <- length_zero_iff_nil in H14. 
-rewrite H14 in H7; rewrite <- H7 in H5; rewrite valubytes_is in H5; omega.
-rewrite H7 in H14; rewrite H5 in H14.
-unfold lt in H.
-rewrite valubytes_is in *; omega.
-
-simpl; auto.
-simpl.
 repeat rewrite app_length.
 rewrite map_length.
 unfold get_sublist.
@@ -1647,39 +2660,41 @@ auto.
 rewrite Nat.add_assoc.
 rewrite Nat.add_sub_assoc.
 rewrite valubytes_is; omega.
+auto.
+
+rewrite Nat.add_assoc.
+rewrite Nat.add_sub_assoc.
+rewrite valubytes_is; omega.
 
 apply list2nmem_arrayN_bound in H9 as H'.
 destruct H'.
-rewrite <- length_zero_iff_nil in H14. 
-rewrite H14 in H7; rewrite <- H7 in H5; rewrite valubytes_is in H5; omega.
-rewrite H7 in H14; rewrite H5 in H14.
-unfold lt in H.
+rewrite <- length_zero_iff_nil in H12. 
+rewrite H12 in H7; rewrite <- H7 in H5; rewrite valubytes_is in H5; omega.
+rewrite H7 in H12; rewrite H5 in H12.
 rewrite valubytes_is in *; omega.
 
 rewrite skipn_length.
 rewrite valubytes_is in *; omega.
-
-apply list2nmem_arrayN_bound in H9 as H'.
-destruct H'.
-rewrite <- length_zero_iff_nil in H14. 
-rewrite H14 in H7; rewrite <- H7 in H5; rewrite valubytes_is in H5; omega.
-rewrite H7 in H14; rewrite H5 in H14.
-unfold lt in H.
 rewrite valubytes_is in *; omega.
 
 repeat split.
 eauto.
+pred_apply.
+cancel.
+instantiate (4:= (updN flist0 inum (BFILE.mk_bfile ((BFILE.BFData f0) ⟦ block_off + m1
+                       := (list2valu (get_sublist data (m1 * valubytes) valubytes), nil) ⟧) (BFILE.BFAttr f0)))).
+instantiate (1:= frees_2).
+instantiate (1:= frees_1).
+instantiate (1:= ilist).
+instantiate (1:= (bxp_1, bxp_2)).
+pred_apply. cancel.
+repeat (split; try rewrite <- plus_n_O; eauto).
+sepauto.
+eauto.
+eauto.
 Admitted.
 
-
-
-
-
-
-
-
-
-
+Hint Extern 1 ({{_}} Bind (write_middle_blocks _ _ _ _ _ _ _) _) => apply write_middle_blocks_ok : prog.
 
 
 Theorem dwrite_middle_blocks_ok : forall lxp bxp ixp inum block_off num_of_full_blocks data fms,
@@ -1800,24 +2815,7 @@ right; omega.
 step.
 Admitted.
 
-Theorem getlen_ok : forall lxp bxp ixp inum fms,
-{< F Fm Fi m0 m flist ilist frees f fy,
-PRE:hm
-       LOG.rep lxp F (LOG.ActiveTxn m0 m) (BFILE.MSLL fms) hm *
-       [[[ m ::: (Fm * BFILE.rep bxp ixp flist ilist frees) ]]] *
-       [[[ flist ::: (Fi * inum |-> f) ]]] *
-       rep f fy
-POST:hm' RET:^(fms',r)
-       LOG.rep lxp F (LOG.ActiveTxn m0 m) (BFILE.MSLL fms') hm' *
-       [[ r = length (ByFData fy)]] *
-       [[ BFILE.MSAlloc fms = BFILE.MSAlloc fms' ]]
-CRASH:hm'  exists fms',
-       LOG.rep lxp F (LOG.ActiveTxn m0 m) (BFILE.MSLL fms') hm'
->} getlen lxp ixp inum fms.
-Proof.
-unfold getlen, rep.
-hoare.
-Qed.
+Hint Extern 1 ({{_}} Bind (dwrite_middle_blocks _ _ _ _ _ _ _) _) => apply dwrite_middle_blocks_ok : prog.
 
 Theorem read_from_block_ok: forall lxp bxp ixp inum fms block_off byte_off read_length,
  {< F Fm Fi Fd m0 m flist ilist frees f fy (data: list byteset),
@@ -1869,7 +2867,7 @@ apply byteset0.
 Qed.
 
 
-
+Hint Extern 1 ({{_}} Bind (read_from_block _ _ _ _ _ _ _) _) => apply read_from_block_ok : prog.
 
 Theorem read_middle_blocks_ok: forall lxp bxp ixp inum fms block_off num_of_full_blocks,
  {< F Fm Fi Fd m0 m flist ilist frees f fy (data: list byteset),
@@ -1962,7 +2960,7 @@ Grab Existential Variables.
 constructor.
 Qed.
 
-
+Hint Extern 1 ({{_}} Bind (read_middle_blocks _ _ _ _ _ _ _) _) => apply read_middle_blocks_ok : prog.
 
 Theorem read_ok : forall lxp bxp ixp inum off len fms,
     {< F Fm Fi Fd m0 m flist ilist frees f fy data,
@@ -2639,190 +3637,5 @@ rewrite H5; reflexivity.
 omega.
 Qed.
 
-Theorem write_first_block_ok : forall lxp bxp ixp inum block_off byte_off data fms,
-    {< F Fm Fi Fd ds flist ilist frees f fy old_data,
-    PRE:hm
-           LOG.rep lxp F (LOG.ActiveTxn ds ds!!) (BFILE.MSLL fms) hm *
-           [[[ ds!! ::: (Fm * BFILE.rep bxp ixp flist ilist frees) ]]] *
-           [[[ flist ::: (Fi * inum |-> f) ]]] *
-           rep f fy  *
-           [[[ (ByFData fy) ::: (Fd * arrayN (ptsto (V:=byteset)) (block_off * valubytes + byte_off) old_data)]]] *
-           [[ length old_data = length data]] *
-           [[ length data > 0 ]] *
-           [[ byte_off + length data <= valubytes ]] 
-           
-     POST:hm' RET:fms'  exists flist' f' ds0 ds',
-           let fy' := mk_bytefile (updN_list (ByFData fy) (block_off * valubytes + byte_off) data) (ByFAttr fy) in  
-           LOG.rep lxp F (LOG.ActiveTxn ds' ds'!!) (BFILE.MSLL fms') hm' *
-           [[ ds' = dsblistupd ds0 (block_off * valubytes + byte_off) (updN_list old_data 0 data) /\ BFILE.diskset_was ds0 ds ]] *
-           [[[ ds'!! ::: (Fm  * BFILE.rep bxp ixp flist' ilist frees) ]]] *
-           [[[ flist' ::: (Fi * inum |-> f') ]]] *
-           rep f' fy' *
-           [[[ (ByFData fy') ::: (Fd * arrayN (ptsto (V:=byteset)) 
-           (block_off * valubytes + byte_off) (updN_list old_data 0 data))]]] *
-           [[ BFILE.MSAlloc fms = BFILE.MSAlloc fms' ]]
-    XCRASH:hm'
-          LOG.recover_any lxp F ds hm' \/
-          LOG.recover_any lxp F (dsblistupd ds (block_off * valubytes + byte_off)  (updN_list old_data 0 data)) hm'
-    >} write_to_block lxp ixp inum fms block_off byte_off data.
-
-Proof.
-unfold write_to_block, rep.
-step.
-
-eapply inlen_bfile; try eauto; try omega.
-
-eapply protobyte2block; eauto.
-eapply unifiedbyte2protobyte with (a:= block_off * valubytes + byte_off) (k:= valubytes) in H19; try omega.
-rewrite div_eq in H19; try omega.
-apply H19.
-
-eapply proto_len; eauto.
-
-eapply byte2unifiedbyte; eauto.
-pred_apply.
-rewrite arrayN_isolate with (i:=0).
-rewrite <- plus_n_O .
-cancel.
-omega.
-
-prestep.
-norm.
-unfold stars; cancel.
-repeat split. 
-
-eapply inlen_bfile; try eauto; try omega.
-eauto.
-eauto.
-
-eapply protobyte2block; eauto.
-eapply unifiedbyte2protobyte with (a:= block_off * valubytes + byte_off) (k:= valubytes) in H19; try omega.
-rewrite div_eq in H19; try omega.
-apply H19.
-
-eapply proto_len; eauto.
-
-eapply byte2unifiedbyte; eauto.
-pred_apply.
-rewrite arrayN_isolate with (i:=0).
-rewrite <- plus_n_O .
-cancel.
-omega.
-
-Focus 5.
-cancel.
-erewrite lift_impl.
-rewrite sep_star_comm; apply H1.
-cancel.
-apply crash_xform_pimpl.
-apply pimpl_or_r.
-rewrite LOG.active_intact.
-left.
-apply LOG.intact_any.
-intros; exists l; auto.
-
-Focus 2.
-auto.
-
-Focus 2.
-step.
-unfold BFILE.block_belong_to_file in H26.
-destruct H26.
-rewrite H12.
-apply arrayN_list2nmem in H8 as H8'.
-rewrite H8'; rewrite H7.
-rewrite H18.
-rewrite <- skipn_firstn_comm.
-rewrite firstn_firstn.
-rewrite Nat.min_l.
-rewrite skipn_firstn_comm.
-
-unfold get_sublist.
-unfold bytesets2valuset.
-unfold list2byteset.
-remember ( bytesets2valuset_rec
-                  (map byteset2list (firstn valubytes (skipn (block_off * valubytes) (UByFData ufy))))
-                  (length
-                     (byteset2list (firstn valubytes (skipn (block_off * valubytes) (UByFData ufy))) ⟦ 0 ⟧))) as c.
-destruct c.
-simpl.
-
-
-
-symmetry in Heqc; apply b2v_rec_nil in Heqc.
-destruct Heqc.
-unfold byteset2list in H13.
-simpl in H13.
-inversion H13.
-apply map_eq_nil in H13.
-apply firstn_is_nil in H13.
-
-
- 
-apply list2nmem_arrayN_bound in H8.
-rewrite bytefile_unified_byte_len with (ufy:=ufy) in H8.
-destruct H8.
-apply length_zero_iff_nil in H8; rewrite <- H7 in H6; rewrite H8 in H6; inversion H6.
-apply le2lt_l in H8.
-apply lt_weaken_l in H8.
-apply skipn_not_nil in H8.
-contradiction.
-omega.
-auto.
-omega.
-
-simpl in *.
-
-destruct (map byteset2list (firstn valubytes (skipn (block_off * valubytes) (UByFData ufy)))) eqn:D.
-inversion Heqc.
-
-
-unfold selN' in *. 
-inversion Heqc.
-rewrite list2valu2list.
-unfold vsmerge.
-simpl.
-rewrite selN_firstn.
-rewrite skipn_selN.
-rewrite <- plus_n_O.
-
-unfold dsblistupd.
-
-destruct (updN_list (firstn (length data) (skipn (block_off * valubytes + byte_off) (ByFData fy))) 0 data) eqn:D1.
-apply updN_list_nil in D1.
-destruct D1.
-rewrite H21 in H6; inversion H6.
-
-fold dsblistupd.
-replace (updN_list (firstn (length data) (skipn (block_off * valubytes + byte_off) (UByFData ufy))) 0 data)
-    with (p :: l3).
-simpl.
-unfold dsbupd.
-unfold ds2llb, llb2ds.
-
-
-destruct ds0.
-repeat (rewrite d_map_d_map; simpl).
-repeat (rewrite map_map; simpl).
-
-replace (fun x : LogReplay.diskstate =>
-      map bytesets2valuset
-        (map (fun x0 : list byteset => x0 ⟦ block_off * valubytes + byte_off := p ⟧) (map valuset2bytesets x)))
-         with (fun x : LogReplay.diskstate =>
-        (map (fun x0 : valuset => bytesets2valuset ((valuset2bytesets x0) ⟦ block_off * valubytes + byte_off := p ⟧)) x)).
-
-Fact bs2vs_updN_vs2bs: forall i bs vs def,
-bytesets2valuset (updN def (valuset2bytesets vs) i bs) = 
-
-unfold d_map.
-simpl.
-destruct ds0.
-
-unfold updN_list in D1.
-destruct data.
-inversion H6.
-
-
-Admitted.
 
 End ABYTEFILE.
